CPSify montgomery wbw reduction
I didn't want to bother redoing all of the proofs that I'd already done,
so instead I prove the cps'ified version equal to the non-cps version,
and transfer over the proofs that way.

src/Arithmetic/MontgomeryReduction/WordByWord/Proofs.v
@@ -6,6 +6,7 @@ Require Import Crypto.Arithmetic.MontgomeryReduction.WordByWord.Abstract.Definit
 Require Import Crypto.Arithmetic.MontgomeryReduction.WordByWord.Abstract.Proofs.
 Require Import Crypto.Arithmetic.MontgomeryReduction.WordByWord.Definition.
 Require Import Crypto.Util.ZUtil.
+Require Import Crypto.Util.Tactics.BreakMatch.
 
 Local Open Scope Z_scope.
 Local Coercion Z.pos : positive >-> Z.
@@ -70,20 +71,98 @@ Section WordByWordMontgomery.
     rewrite Znat.Nat2Z.inj_succ, Z.pow_succ_r by lia; reflexivity.
   Qed.
 
+  Local Notation redc_body_no_cps := (@redc_body_no_cps r R_numlimbs N).
+  Local Notation redc_body_cps := (@redc_body_cps r R_numlimbs N).
+  Local Notation redc_body := (@redc_body r R_numlimbs N).
+  Local Notation redc_loop_no_cps := (@redc_loop_no_cps r R_numlimbs N B k).
+  Local Notation redc_loop_cps := (@redc_loop_cps r R_numlimbs N B k).
+  Local Notation redc_loop := (@redc_loop r R_numlimbs N B k).
+  Local Notation redc_no_cps := (@redc_no_cps r R_numlimbs N A B k).
+  Local Notation redc_cps := (@redc_cps r R_numlimbs N A B k).
   Local Notation redc := (@redc r R_numlimbs N A B k).
 
-  Definition redc_bound : 0 <= eval redc < eval N + eval B
+  Definition redc_no_cps_bound : 0 <= eval redc_no_cps < eval N + eval B
     := @redc_bound T eval numlimbs zero divmod r r_big small eval_zero eval_div eval_mod small_div scmul eval_scmul R R_numlimbs R_correct add eval_add small_add drop_high eval_drop_high N Npos Npos_correct N_lt_R B B_bound ri k A small_A.
-  Definition numlimbs_redc_gen
-    : numlimbs redc
+  Definition numlimbs_redc_no_cps_gen
+    : numlimbs redc_no_cps
       = match numlimbs A with
         | O => S (numlimbs B)
         | _ => S R_numlimbs
         end
     := @numlimbs_redc_gen T eval numlimbs zero divmod r r_big small eval_zero numlimbs_zero eval_div eval_mod small_div numlimbs_div scmul eval_scmul numlimbs_scmul R R_numlimbs R_correct add eval_add small_add numlimbs_add drop_high eval_drop_high numlimbs_drop_high N Npos Npos_correct N_lt_R B B_bound ri k A small_A Hnumlimbs_le.
-  Definition numlimbs_redc : numlimbs redc = S (numlimbs B)
+  Definition numlimbs_redc_no_cps : numlimbs redc_no_cps = S (numlimbs B)
     := @numlimbs_redc T eval numlimbs zero divmod r r_big small eval_zero numlimbs_zero eval_div eval_mod small_div numlimbs_div scmul eval_scmul numlimbs_scmul R R_numlimbs R_correct add eval_add small_add numlimbs_add drop_high eval_drop_high numlimbs_drop_high N Npos Npos_correct N_lt_R B B_bound ri k A small_A Hnumlimbs_eq.
-  Definition redc_mod_N
-    : (eval redc) mod (eval N) = (eval A * eval B * ri^(Z.of_nat (numlimbs A))) mod (eval N)
+  Definition redc_no_cps_mod_N
+    : (eval redc_no_cps) mod (eval N) = (eval A * eval B * ri^(Z.of_nat (numlimbs A))) mod (eval N)
     := @redc_mod_N T eval numlimbs zero divmod r r_big small eval_zero eval_div eval_mod small_div scmul eval_scmul R R_numlimbs R_correct add eval_add small_add drop_high eval_drop_high N Npos Npos_correct N_lt_R B B_bound ri ri_correct k k_correct A small_A A_bound.
+
+  Lemma redc_body_cps_id (A' S' : T) {cpsT} f
+    : @redc_body_cps A' B k S' cpsT f = f (redc_body A' B k S').
+  Proof.
+    unfold redc_body, redc_body_cps, LetIn.Let_In.
+    repeat first [ reflexivity
+                 | break_innermost_match_step
+                 | progress autorewrite with uncps ].
+  Qed.
+
+  Lemma redc_loop_cps_id (count : nat) (A_S : T * T) {cpsT} f
+    : @redc_loop_cps cpsT count f A_S = f (redc_loop count A_S).
+  Proof.
+    unfold redc_loop.
+    revert A_S f.
+    induction count as [|count IHcount].
+    { reflexivity. }
+    { intros [A' S']; simpl; intros.
+      etransitivity; rewrite @redc_body_cps_id; [ rewrite IHcount | ]; reflexivity. }
+  Qed.
+  Lemma redc_cps_id {cpsT} f : @redc_cps cpsT f = f redc.
+  Proof.
+    unfold redc, redc_cps.
+    etransitivity; rewrite redc_loop_cps_id; [ | reflexivity ]; break_innermost_match; reflexivity.
+  Qed.
+
+  Lemma redc_body_id_no_cps A' S'
+    : redc_body A' B k S' = redc_body_no_cps B k (A', S').
+  Proof.
+    unfold redc_body, redc_body_cps, redc_body_no_cps, Abstract.Definition.redc_body, LetIn.Let_In, id.
+    repeat autounfold with word_by_word_montgomery.
+    repeat first [ reflexivity
+                 | progress cbn [fst snd id]
+                 | progress autorewrite with uncps
+                 | break_innermost_match_step
+                 | f_equal; [] ].
+  Qed.
+  Lemma redc_loop_cps_id_no_cps count A_S
+    : redc_loop count A_S = redc_loop_no_cps count A_S.
+  Proof.
+    unfold redc_loop_no_cps, id.
+    revert A_S.
+    induction count as [|count IHcount]; simpl; [ reflexivity | ].
+    intros [A' S']; unfold redc_loop; simpl.
+    rewrite redc_body_cps_id, redc_loop_cps_id, IHcount, redc_body_id_no_cps.
+    reflexivity.
+  Qed.
+  Lemma redc_cps_id_no_cps : redc = redc_no_cps.
+  Proof.
+    unfold redc, redc_no_cps, redc_cps, Abstract.Definition.redc.
+    rewrite redc_loop_cps_id, (surjective_pairing (redc_loop _ _)).
+    rewrite redc_loop_cps_id_no_cps; reflexivity.
+  Qed.
+
+  Lemma redc_bound : 0 <= eval redc < eval N + eval B.
+  Proof. rewrite redc_cps_id_no_cps; apply redc_no_cps_bound. Qed.
+  Lemma numlimbs_redc_gen
+    : numlimbs redc
+      = match numlimbs A with
+        | O => S (numlimbs B)
+        | _ => S R_numlimbs
+        end.
+  Proof. rewrite redc_cps_id_no_cps; apply numlimbs_redc_no_cps_gen. Qed.
+  Lemma numlimbs_redc : numlimbs redc = S (numlimbs B).
+  Proof. rewrite redc_cps_id_no_cps; apply numlimbs_redc_no_cps. Qed.
+  Lemma redc_mod_N
+    : (eval redc) mod (eval N) = (eval A * eval B * ri^(Z.of_nat (numlimbs A))) mod (eval N).
+  Proof. rewrite redc_cps_id_no_cps; apply redc_no_cps_mod_N. Qed.
 End WordByWordMontgomery.
+
+Hint Rewrite redc_body_cps_id redc_loop_cps_id redc_cps_id : uncps.
